src/TypEnv.v
@@ -21,6 +21,8 @@ Module TypEnv.
 
   Definition find (v : var) (e : t) : option typ := VM.find v e.
 
+  Definition mem (v : var) (e : t) : bool := VM.mem v e.
+
   Definition add (v : var) (ty : typ) (e : t) := VM.add v ty e.
 
   Lemma find_add_eq {x y ty e} : x == y -> find x (add y ty e) = Some ty.
@@ -28,5 +30,20 @@ Module TypEnv.
 
   Lemma find_add_neq {x y ty e} : x != y -> find x (add y ty e) = find x e.
   Proof. move/negP=> Hxy. exact: (VM.Lemmas.find_add_neq Hxy). Qed.
+
+  Lemma mem_find_some v e : mem v e -> exists ty, find v e = Some ty.
+  Proof. exact: VM.Lemmas.mem_find_some. Qed.
+
+  Lemma not_mem_find_none v e : ~~ mem v e -> find v e = None.
+  Proof. exact: VM.Lemmas.not_mem_find_none. Qed.
+
+  Lemma mem_add_eq {x y ty e} : x == y -> mem x (add y ty e).
+  Proof. exact: VM.Lemmas.mem_add_eq. Qed.
+
+  Lemma mem_add_neq {x y ty e} : x != y -> mem x (add y ty e) = mem x e.
+  Proof. move/idP/negP=> H. exact: (VM.Lemmas.mem_add_neq H). Qed.
+
+  Lemma find_some_vsize x e ty : find x e = Some ty -> vsize x e = sizeof_typ ty.
+  Proof. rewrite /vsize /find. move=> ->. reflexivity. Qed.
 
 End TypEnv.
